@prefix rdf: <http://www.w3.org/1999/02/22-rdf-syntax-ns#> .
@prefix holding: <http://purl.org/ontology/holding#> .
@prefix bf: <http://bibframe.org/vocab/> .
@prefix bibo: <http://purl.org/ontology/bibo/> .
@prefix cc: <http://creativecommons.org/ns#> .
@prefix daia: <http://purl.org/ontology/daia/> .
@prefix dct: <http://purl.org/dc/terms/> .
@prefix dso: <http://purl.org/ontology/dso#> .
@prefix ecpo: <http://purl.org/ontology/ecpo#> .
@prefix foaf: <http://xmlns.com/foaf/0.1/> .
@prefix frbr: <http://purl.org/vocab/frbr/core#> .
@prefix gr: <http://purl.org/goodrelations/v1#> .
@prefix org: <http://www.w3.org/ns/org#> .
@prefix owl: <http://www.w3.org/2002/07/owl#> .
@prefix rdfs: <http://www.w3.org/2000/01/rdf-schema#> .
@prefix schema: <http://schema.org/> .
@prefix service: <http://purl.org/ontology/service#> .
@prefix skos: <http://www.w3.org/2004/02/skos/core#> .
@prefix ssso: <http://purl.org/ontology/ssso#> .
@prefix vann: <http://purl.org/vocab/vann/> .
@prefix xsd: <http://www.w3.org/2001/XMLSchema#> .

gr:Location
    a owl:Class ;
    rdfs:isDefinedBy <http://purl.org/goodrelations/v1> ;
    rdfs:label "Location"@en ;
    owl:equivalentClass schema:Place .

gr:availableAtOrFrom
    a owl:AnnotationProperty ;
    rdfs:isDefinedBy <http://purl.org/goodrelations/v1> ;
    skos:scopeNote "Used to relate a document service offered for an item with a location."@en .

gr:hasStockKeepingUnit
    a owl:AnnotationProperty ;
    rdfs:isDefinedBy <http://purl.org/goodrelations/v1> ;
    rdfs:seeAlso schema:sku ;
    skos:scopeNote "Used to identify the item for which a document service is offered."@en .

gr:name
    a owl:AnnotationProperty ;
    rdfs:isDefinedBy <http://purl.org/goodrelations/v1> ;
    skos:scopeNote "When a document service is offered for an item, this property is used to name the location where the document service should be provided."@en .

bibo:Document
    a owl:Class ;
    rdfs:isDefinedBy <http://purl.org/ontology/bibo/> ;
    rdfs:label "Document"@en ;
    rdfs:seeAlso bf:Work ;
    owl:equivalentClass foaf:Document .

dso:DocumentService
    a owl:Class ;
    rdfs:isDefinedBy <http://purl.org/ontology/dso> ;
    rdfs:label "DocumentService" .

ecpo:Chronology
    a owl:Class ;
    rdfs:isDefinedBy <http://purl.org/ontology/ecpo> ;
    rdfs:label "Chronology"@en .

<http://purl.org/ontology/holding>
    cc:license <http://creativecommons.org/licenses/by/3.0/> ;
    dct:creator "Carsten Klee", "Jakob Vo√ü" ;
    dct:modified "2014-01-10"^^xsd:date ;
    dct:title "Holding Ontology"@en ;
    vann:preferredNamespacePrefix "holding" ;
    vann:preferredNamespaceUri "http://purl.org/ontology/holding#" ;
    a owl:Ontology ;
    rdfs:label "Holding Ontology"@en ;
    owl:versionInfo "0.1.2" .

holding:broaderExemplar
    a owl:ObjectProperty ;
    rdfs:comment "Relates a Document to an Item that contains an exemplar of the Document as part."@en ;
    rdfs:domain bibo:Document ;
    rdfs:label "broader exemplar"@en ;
    rdfs:range frbr:Item ;
    owl:inverseOf holding:broaderExemplarOf .

holding:broaderExemplarOf
    a owl:ObjectProperty ;
    rdfs:comment "Relates an Item to a Document which is partly exemplified by the Item."@en ;
    rdfs:domain frbr:Item ;
    rdfs:label "broader exemplar of"@en ;
    rdfs:range bibo:Document ;
    owl:inverseOf holding:broaderExemplar .

holding:exemplar
    a owl:ObjectProperty ;
    rdfs:comment "Relates a Document to an Item that is an exemplar of the Document. This property is similar to frbr:exemplar but does not refer to the class frbr:Manifestation."@en ;
    rdfs:domain bibo:Document ;
    rdfs:label "has exemplar"@en ;
    rdfs:range frbr:Item ;
    owl:inverseOf holding:exemplarOf .

holding:exemplarOf
    a owl:ObjectProperty ;
    rdfs:comment "Relates an Item to the Document that is exemplified by the Item."@en ;
    rdfs:domain frbr:Item ;
    rdfs:label "is examplar of"@en ;
    rdfs:range bibo:Document ;
    owl:inverseOf holding:exemplar .

holding:heldBy
    a owl:ObjectProperty ;
    rdfs:comment "Relates an item to an agent who holds the item."@en ;
    rdfs:domain frbr:Item ;
    rdfs:label "held by"@en ;
    rdfs:range foaf:Agent ;
    rdfs:subPropertyOf holding:collectedBy ;
    owl:inverseOf holding:holds .

holding:holds
    a owl:ObjectProperty ;
    rdfs:comment "Relates an agent to an item which the agent holds."@en ;
    rdfs:domain foaf:Agent ;
    rdfs:label "holds"@en ;
    rdfs:range frbr:Item ;
    owl:inverseOf holding:heldBy .

holding:label
    a owl:DatatypeProperty ;
    rdfs:comment "A call number, shelf mark or similar label of an item"@en ;
    rdfs:domain frbr:Item ;
    rdfs:label "label"@en ;
    rdfs:range rdfs:Literal ;
    rdfs:subPropertyOf dct:identifier .

holding:narrowerExemplar
    a owl:ObjectProperty ;
    rdfs:comment "Relates an Item to a Document which is partly exemplified by the Item."@en ;
    rdfs:domain frbr:Item ;
    rdfs:label "narrower exemplar"@en ;
    rdfs:range bibo:Document ;
    owl:inverseOf holding:narrowerExemplarOf .

holding:narrowerExemplarOf
    a owl:ObjectProperty ;
    rdfs:comment "Relates a Document to an Item that is an exemplar of a part of the Document."@en ;
    rdfs:domain bibo:Document ;
    rdfs:label "narrower exemplar of"@en ;
    rdfs:range frbr:Item ;
    owl:inverseOf holding:narrowerExemplar .

service:providedBy
    a owl:AnnotationProperty ;
    rdfs:isDefinedBy <http://purl.org/ontology/service> ;
    skos:scopeNote "Used to relate a document service with an agent who offered the service." .

frbr:Item
    a owl:Class ;
    rdfs:isDefinedBy <http://purl.org/vocab/frbr/core> ;
    rdfs:label "Item"@en ;
    rdfs:seeAlso bf:Instance .

org:siteOf
    a owl:AnnotationProperty ;
    rdfs:isDefinedBy <http://www.w3.org/ns/org> ;
    skos:scopeNote "This property is used to relate a location with an agent."@en .

foaf:Agent
    a owl:Class ;
    rdfs:isDefinedBy <http://xmlns.com/foaf/0.1/> ;
    rdfs:label "Agent"@en ;
    rdfs:seeAlso bf:Agent .

